Change the state to "int=>int", and the definition of assn and com, with the proof_system, haven't finished yet.

Ann_Com.thy
@@ -2,23 +2,35 @@ theory Ann_Com
 imports BExp
 begin
 
-type_synonym assn = "state \<Rightarrow> bool"
+type_synonym address = int
+type_synonym newstate = "address \<Rightarrow> int"
+
+type_synonym assn = "newstate \<Rightarrow> bool"
 
 datatype com =
-  Basic "state \<Rightarrow> state"      |
+  Basic "newstate \<Rightarrow> newstate"      |
   Seq   com com          ("_;; _") |
-  Cond "state \<Rightarrow> bool" com com      ("IF _ THEN _ ELSE _ FI")|
-  While bexp assn com    ("WHILE _ INV _ DO _ OD")|
-  Wait bexp              ("WAIT _ END")
+  Cond "newstate \<Rightarrow> bool" com com      ("IF _ THEN _ ELSE _ FI")|
+  While "newstate \<Rightarrow> bool" assn com    ("WHILE _ INV _ DO _ OD")|
+  Wait "newstate \<Rightarrow> bool"              ("WAIT _ END")
 
-term "IF (\<lambda> s . s ''x'' = 1) THEN Basic id ELSE Basic id FI"
+fun list :: "newstate \<Rightarrow> (int list) \<Rightarrow> int \<Rightarrow> bool" where 
+"list s [] i = (i = 0)"|
+"list s (x#xs) i = (\<exists>j. (s i = x) \<and> (s (i + 1) = j) \<and> list s xs j)"
+
+fun reach_step::"newstate \<Rightarrow> nat \<Rightarrow> int \<Rightarrow> int \<Rightarrow> bool" where
+"reach_step s 0 i j = (i = j)"|
+"reach_step s (Suc n) i j = (\<exists>a k. (s i = a) \<and> (s (i + 1) = k) \<and> (reach_step s n k j))"
+
+definition reach::"newstate \<Rightarrow> int \<Rightarrow> int \<Rightarrow> bool" where
+  "reach s i j \<equiv> (\<exists>n \<ge> 0. reach_step s n i j)"
 
 datatype acom =
-  ABasic assn "state \<Rightarrow> state"      |
+  ABasic assn "newstate \<Rightarrow> newstate"      |
   ASeq   acom acom   ("_;; _") |
-  ACond assn bexp acom acom     ("{_} IF _ THEN _ ELSE _ FI")|
-  AWhile assn bexp assn acom    ("{_} WHILE _ INV _ DO _ OD")|
-  AWait assn bexp              ("{_} WAIT _ END")
+  ACond assn "newstate \<Rightarrow> bool" acom acom     ("{_} IF _ THEN _ ELSE _ FI")|
+  AWhile assn "newstate \<Rightarrow> bool" assn acom    ("{_} WHILE _ INV _ DO _ OD")|
+  AWait assn "newstate \<Rightarrow> bool"              ("{_} WAIT _ END")
 
 fun pre :: "acom \<Rightarrow> assn" where
 "pre (ABasic P f) = P" |
